$$
u_1=\sin(\pi x)\sin(\pi y)\sin(\pi t)
$$

$$
u_2=x(x-1)y(y-1)\cos(t)
$$

对于PDE:
$$
\begin{aligned}
&\mathbf{u}_{t t}-\nabla \cdot \sigma(\mathbf{u})=\mathbf{f} \; \text{in} \;\Omega\times [0,T]\\
&\mathbf{u}=\mathbf{g} \; \text{on}\; \partial \Omega \times [0,T]\\
&\mathbf{u}=\mathbf{u}_0,\; \frac{\partial \mathbf{u}}{\partial t}=\mathbf{u}_{00}\;
\text{at}\; t=0 \; \text{and}\; \text{in} \; \Omega
\end{aligned}
$$

$$
\frac{\partial u_1}{\partial x}=\pi  \sin (\pi  t) \cos (\pi  x) \sin (\pi  y)
$$

$$
\frac{\partial u_1}{\partial y}=\pi  \sin (\pi  t) \sin (\pi  x) \cos (\pi  y)
$$

$$
\frac{\partial u_2}{\partial x}=(2 x-1) (y-1) y \cos (t)
$$

$$
\frac{\partial u_2}{\partial y}=(-1 + x) x (-1 + 2 y) \cos(t)
$$


$$
f_1=\pi ^2 (\lambda +3 \mu -1) \sin (\pi  t) \sin (\pi  x) \sin (\pi  y)-(2 x-1) (2 y-1) (\lambda +\mu ) \cos (t)\\
$$

$$
\begin{aligned}
f_2=&\cos (t) \left(2 \mu  \left(-2 (x-1) x-y^2+y\right)-(x-1) x (2 \lambda +(y-1) y)\right)\\
&-\pi ^2 (\lambda +\mu ) \sin (\pi  t) \cos (\pi  x) \cos (\pi  y)
\end{aligned}
$$



初始条件：
$$
\begin{aligned}
&u_1(0)=0,u_2(0)=(2 x-1) (y-1) y\\
&\frac{\partial u_1}{\partial t}​=\pi  \sin (\pi  x) \sin (\pi  y)​\\
&\frac{\partial u_2}{\partial t} =0
\end{aligned}
$$
边界条件（[-1,1]$\times$[-1,1]）：
$$
u_1=0;
$$

$$
\begin{aligned}
x=-1,u_2&=2 (y-1) y \cos (t)\\
x=1,u_2&=0\\
y=-1,u_2&=2 (x-1) x \cos (t)\\
y=1,u_2&=0
\end{aligned}
$$

